\documentclass{article}
\usepackage{amsmath,amsfonts,amsthm}

\usepackage{bbold}

\newtheorem{definition}{Definition}
\newtheorem{lemma}{Lemma}

\DeclareMathOperator{\sign}{sign}

\begin{document}

\begin{definition}
\begin{eqnarray*}
  \phi(x) & = & \frac{1}{\sqrt{2\pi}}\exp\left(-\frac{x^2}{2}\right)\\
\end{eqnarray*}
\end{definition}

\begin{definition}
  \begin{eqnarray*}
    \sigma_i & = & \exp\left( \sum_{j=0}^\infty a_j \epsilon_{i-j} + \mu\right)\\
    R_i & = & \sigma_i \delta_i\\
    V_i & = & \exp\left(V_{i-1} + R_i\right)\\
  \end{eqnarray*}

  where $\epsilon$, $\delta$ are distributione IID $N(0,1)$\\
\end{definition}

\begin{lemma}
  {\em (Change of variables for probability densities)}
  If $g$ is monotonic:
  
  \begin{eqnarray*}
    f_{g(X)}(y) = \frac{f_X\left(g^{-1}(y)\right)}{\left|\det\left(\frac{d\!g}{d\!x}(x)\right)\right|}
  \end{eqnarray*}
\end{lemma}

\begin{lemma}
  \begin{eqnarray*}
    \det\left(\begin{array}{cc}
      I & 0\\
      M & N\\
    \end{array}\right) = \det N
  \end{eqnarray*}
\end{lemma}

\begin{lemma}
  \begin{eqnarray*}
    f_{\epsilon,R}\left(\epsilon,R\right) = \frac{\prod_i \phi\left( \frac{R_i}{\exp\left(\sum_{k=0}^\infty a_k \epsilon_{i-k} + \mu\right)}\right)}{\exp\left(\sum_i \left(\sum_{k=0}^\infty a_k \epsilon_{i-k} + \mu\right)\right)}\\
  \end{eqnarray*}
\end{lemma}
\begin{proof}
  Define:

  \begin{eqnarray*}
    g(\epsilon, \delta) = \left(\epsilon, R\right)
  \end{eqnarray*}

  Now:

  \begin{eqnarray*}
    \frac{d\!R_i}{d\!\delta_j} = \exp\left(\sum_{k=0}^\infty a_k\epsilon_{i-k} + \mu\right) \mathbb{1}_{i=j}
  \end{eqnarray*}

  and:

  \begin{eqnarray*}
    \frac{d\!\epsilon}{d\!\delta} = 0\\
    \frac{d\!\epsilon}{d\!\epsilon} = I\\
  \end{eqnarray*}

  so that:

  \begin{eqnarray*}
    \det\left(\frac{d\!g}{d\!x}(x)\right) & = & \prod_i \frac{d\!R_i}{d\!\delta_i} = \prod_i \exp\left(\sum_{k=0}^\infty a_k \epsilon_{i-k} + \mu\right)\\
    & = & \exp\left(\sum_i \left(\sum_{k=0}^\infty a_k \epsilon_{i-k} + \mu\right)\right)\\
  \end{eqnarray*}

  Hence:

  \begin{eqnarray*}
    f_{\epsilon,R}\left(\epsilon,R\right) = \frac{\prod_i \phi\left( \frac{R_i}{\exp\left(\sum_{k=0}^\infty a_k \epsilon_{i-k} + \mu\right)}\right)}{\exp\left(\sum_i \left(\sum_{k=0}^\infty a_k \epsilon_{i-k} + \mu\right)\right)}\\
  \end{eqnarray*}
\end{proof}

\begin{lemma}
  \begin{eqnarray*}
    E_{a',\mu'}\left[\left. \log f_{\epsilon,R}\left(\epsilon,R\right) \right| R \right] = 
  \end{eqnarray*}
\end{lemma}
\begin{proof}
  \begin{eqnarray*}
    \lefteqn{\log f_{\epsilon,R}\left(\epsilon,R\right)}\\
    & = & \sum_i \log \phi\left( \frac{R_i}{\exp\left(\sum_{k=0}^\infty a_k \epsilon_{i-k} + \mu\right)}\right) - \sum_i \left(\sum_{k=0}^\infty a_k \epsilon_{i-k} - \mu\right)\\
    & = & -\frac{n}{2} \log\left(2 \pi\right) - \sum_i \frac{1}{2}\left( \frac{R_i}{\exp\left(\sum_{k=0}^\infty a_k \epsilon_{i-k} + \mu\right)}\right)^2 - \sum_i \left(\sum_{k=0}^\infty a_k \epsilon_{i-k} - \mu\right)\\
  \end{eqnarray*}
\end{proof}

\end{document}
